\section{Newton's linearization of~(\ref{first-DS2}) with  (\ref{eq:toto1-ter}) }   \begin{equation}    \begin{array}{l}      \label{eq:full-toto1-ter}      M x_{k+1} = M x_{k} +h \theta f(x_{k+1},t_{k+1}) +h(1-\theta)f(x_{k},t_{k}) + h r_{k+\gamma} \\[2mm]      y_{k+\gamma} =  h(t_{k+\gamma},x_{k+\gamma},\lambda _{k+\gamma}) \\[2mm]      r_{k+\gamma} = g(\lambda_{k+\gamma},t_{k+\gamma})\\[2mm]    \end{array}\end{equation} \paragraph{Newton's linearization of the first line of~(\ref{eq:full-toto1-ter})} The first line of the  problem~(\ref{eq:full-toto1}) can be written under the form of a residue $\mathcal R$ depending only on $x_{k+1}$ and $r_{k+\gamma}$ such that \begin{equation}  \label{eq:full-NL3}  \mathcal R (x_{k+1},r _{k+\gamma}) =0\end{equation}with $\mathcal R(x,r) = M(x - x_{k}) -h\theta f( x , t_{k+1}) - h(1-\theta)f(x_k,t_k) - h r $The solution of this system of nonlinear equations is sought as a limit of the sequence $\{ x^{\alpha}_{k+1},r^{\alpha}_{k+\gamma} \}_{\alpha \in \NN}$ such that \begin{equation}   \label{eq:full-NL7}   \begin{cases}     x^{0}_{k+1} = x_k \\ \\     \mathcal R_L( x^{\alpha+1}_{k+1},r^{\alpha+1}_{k+1}) = \mathcal     R(x^{\alpha}_{k+1},r^{\alpha}_{k+1})  + \left[ \nabla_{x} \mathcal     R(x^{\alpha}_{k+1},r^{\alpha}_{k+1})\right] (x^{\alpha+1}_{k+1}-x^{\alpha}_{k+1} ) +     \left[ \nabla_{r} \mathcal R(x^{\alpha}_{k+1},r^{\alpha}_{k+\gamma})\right] (r^{\alpha+1}_{k+\gamma} - r^{\alpha}_{k+\gamma} ) =0 \end{cases}\end{equation}\begin{ndrva}  What about $r^0_{k+\gamma}$ ?\end{ndrva}The residu free is also defined (useful for implementation only):\[\mathcal R _{free}(x) \stackrel{\Delta}{=}  M(x - x_{k}) -h\theta f( x , t_{k+1}) - h(1-\theta)f(x_k,t_k),\]which yields\[\mathcal R (x,r) = \mathcal R _{free}(x)   - h r .\]\begin{equation}  \mathcal R (x^{\alpha}_{k+1},r^{\alpha}_{k+\gamma}) = \fbox{$\mathcal R^{\alpha}_{k+1} \stackrel{\Delta}{=}  \mathcal R_{free}(x^{\alpha}_{k+1} )  - h r^{\alpha}_{k+\gamma}$}\label{eq:full-rfree-1}\end{equation}\[  \mathcal R_{free}(x^{\alpha}_{k+1} )=\fbox{$ \mathcal R _{free k+1} ^{\alpha} \stackrel{\Delta}{=}  M(x^{\alpha}_{k+1} - x_{k}) -h\theta f( x^{\alpha}_{k+1} , t_{k+1}) - h(1-\theta)f(x_k,t_k)$}\] The computation of the Jacobian of $\mathcal R$ with respect to $x$, denoted by $   W^{\alpha}_{k+1}$ leads to \begin{equation}   \label{eq:full-NL9}   \begin{array}{l}    W^{\alpha}_{k+1} \stackrel{\Delta}{=} \nabla_{x} \mathcal R (x^{\alpha}_{k+1},r^{\alpha}_{k+1})= M - h  \theta \nabla_{x} f(  x^{\alpha}_{k+1}, t_{k+1} ).\\ \end{array}\end{equation}At each time--step, we have to solve the following linearized problem,\begin{equation}   \label{eq:full-NL10}    \mathcal R^{\alpha}_{k+1} + W^{\alpha}_{k+1} (x^{\alpha+1}_{k+1} -    x^{\alpha}_{k+1}) - h  (r^{\alpha+1}_{k+\gamma} - r^{\alpha}_{k+\gamma} )  =0 ,\end{equation}By using (\ref{eq:full-rfree-1}), we get\begin{equation}  \label{eq:full-rfree-2}  \mathcal R _{free}(x^{\alpha}_{k+1})  - h  r^{\alpha+1}_{k+\gamma}   + W^{\alpha}_{k+1} (x^{\alpha+1}_{k+1} -    x^{\alpha}_{k+1})  =0 \end{equation}%\fbox{  \begin{equation}    \boxed{ x^{\alpha+1}_{k+1} = h(W^{\alpha}_{k+1})^{-1}r^{\alpha+1}_{k+1} +x^\alpha_{free}}  \end{equation}}with :\begin{equation}  \boxed{x^\alpha_{free}\stackrel{\Delta}{=}x^{\alpha}_{k+1}-(W^{\alpha}_{k+1})^{-1}\mathcal R_{freek+1}^{\alpha} \label{eq:full-rfree-12}}\end{equation}The matrix $W$ is clearly non singular for small $h$. \paragraph{Newton's linearization of the second  line of~(\ref{eq:full-toto1})}The same operation is performed with the second equation of (\ref{eq:full-toto1})\begin{equation}  \begin{array}{l}    \mathcal R_y(x,y,\lambda)=y-h(t_{k+\gamma},\gamma x + (1-\gamma) x_k ,\lambda) =0\\ \\  \end{array}\end{equation}which is linearized as\begin{equation}  \label{eq:full-NL9}  \begin{array}{l}    \mathcal R_{Ly}(x^{\alpha+1}_{k+1},y^{\alpha+1}_{k+\gamma},\lambda^{\alpha+1}_{k+\gamma}) = \mathcal    R_{y}(x^{\alpha}_{k+1},y^{\alpha}_{k+\gamma},\lambda^{\alpha}_{k+\gamma}) +    (y^{\alpha+1}_{k+\gamma}-y^{\alpha}_{k+\gamma})- \\[2mm] \qquad  \qquad \qquad \qquad  \qquad \qquad    \gamma C^{\alpha}_{k+1}(x^{\alpha+1}_{k+1}-x^{\alpha}_{k+1}) - D^{\alpha}_{k+\gamma}(\lambda^{\alpha+1}_{k+\gamma}-\lambda^{\alpha}_{k+\gamma})=0  \end{array}\end{equation}This leads to the following linear equation\begin{equation}  \boxed{y^{\alpha+1}_{k+\gamma} =  y^{\alpha}_{k+\gamma}  -\mathcal R^{\alpha}_{y,k+1}+ \\  C^{\alpha}_{k+1}(x^{\alpha+1}_{k+1}-x^{\alpha}_{k+1}) +  D^{\alpha}_{k+\gamma}(\lambda^{\alpha+1}_{k+\gamma}-\lambda^{\alpha}_{k+\gamma})}. \label{eq:full-NL11y}\end{equation}with,\begin{equation}     \begin{array}{l}  C^{\alpha}_{k+1} = \nabla_xh(t_{k+1}, x^{\alpha}_{k+1},\lambda^{\alpha}_{k+\gamma} ) \\ \\  D^{\alpha}_{k+\gamma} = \nabla_{\lambda}h(t_{k+1}, x^{\alpha}_{k+1},\lambda^{\alpha}_{k+\gamma}) \end{array}\end{equation}and\begin{equation}\fbox{$\mathcal R^{\alpha}_{yk+1} \stackrel{\Delta}{=} y^{\alpha}_{k+\gamma} - h(x^{\alpha}_{k+1},\lambda^{\alpha}_{k+\gamma})$} \end{equation} \paragraph{Newton's linearization of the third  line of~(\ref{eq:full-toto1})}The same operation is performed with the third equation of (\ref{eq:full-toto1})\begin{equation}  \begin{array}{l}    \mathcal R_r(r,\lambda)=r-g(\lambda,t_{k+1}) =0\\ \\  \end{array}\end{equation}which is linearized as\begin{equation}  \label{eq:full-NL9}  \begin{array}{l}      \mathcal R_{L\lambda}(r^{\alpha+1}_{k+\gamma},\lambda^{\alpha+1}_{k+\gamma}) = \mathcal      R_{rk+\gamma}^{\alpha} + (r^{\alpha+1}_{k+\gamma} - r^{\alpha}_{k+\gamma}) - B^{\alpha}_{k+\gamma}(\lambda^{\alpha+1}_{k+\gamma} -      \lambda^{\alpha}_{k+\gamma})=0    \end{array}  \end{equation}\begin{equation}  \label{eq:full-rrL}  \begin{array}{l}    \boxed{r^{\alpha+1}_{k+\gamma} = g(\lambda ^{\alpha}_{k+\gamma},t_{k+\gamma}) -B^{\alpha}_{k+\gamma}      \lambda^{\alpha}_{k+\gamma} + B^{\alpha}_{k+\gamma} \lambda^{\alpha+1}_{k+\gamma}}         \end{array}\end{equation}with,\begin{equation}     \begin{array}{l}  B^{\alpha}_{k+\gamma} = \nabla_{\lambda}g(\lambda ^{\alpha}_{k+\gamma},t_{k+\gamma}) \end{array}\end{equation}and the  residue for $r$:\begin{equation}\boxed{\mathcal      R_{rk+\gamma}^{\alpha} = r^{\alpha}_{k+\gamma} - g(\lambda ^{\alpha}_{k+\gamma},t_{k+\gamma})}  \end{equation}  \begin{ndrva}    stop here  \end{ndrva}\paragraph{Reduction to a linear relation between  $x^{\alpha+1}_{k+1}$ and$\lambda^{\alpha+1}_{k+\gamma}$}Inserting (\ref{eq:full-rrL}) into~(\ref{eq:full-rfree-12}), we get the following linear relation between $x^{\alpha+1}_{k+1}$ and$\lambda^{\alpha+1}_{k+1}$, \begin{equation}   \begin{array}{l}     x^{\alpha+1}_{k+1} = h\gamma(W^{\alpha}_{k+1} )^{-1}\left[g(x^{\alpha}_{k+1},\lambda^{\alpha}_{k+1},t_{k+1}) +    B^{\alpha}_{k+1} (\lambda^{\alpha+1}_{k+1} - \lambda^{\alpha}_{k+1})+K^{\alpha}_{k+1}    (x^{\alpha+1}_{k+1} - x^{\alpha}_{k+1}) \right ] +x^\alpha_{free}\end{array}\end{equation}that is \begin{equation}  \begin{array}{l}    (I-h \gamma (W^{\alpha}_{k+1})^{-1}K^{\alpha}_{k+1})x^{\alpha+1}_{k+1}=x_p + h \gamma (W^{\alpha}_{k+1})^{-1}    B^{\alpha}_{k+1} \lambda^{\alpha+1}_{k+1}   \end{array}\end{equation}with \begin{equation}  \boxed{x_p \stackrel{\Delta}{=}  h\gamma(W^{\alpha}_{k+1} )^{-1}\left[g(x^{\alpha}_{k+1},\lambda^{\alpha}_{k+1},t_{k+1}) +    -B^{\alpha}_{k+1} (\lambda^{\alpha}_{k+1})-K^{\alpha}_{k+1} (x^{\alpha}_{k+1}) \right ] +x^\alpha_{free}}\end{equation}Let us  define the new matrix\begin{equation}\hat K^{\alpha}_{k+1}=(I-h \gamma (W^{\alpha}_{k+1})K^{\alpha}_{k+1}).\label{eq:full-hatW}\end{equation}We get the linear relation\begin{equation}  \label{eq:full-rfree-13}  \begin{array}{l} \boxed{   x^{\alpha+1}_{k+1}\stackrel{\Delta}{=} \hat K^{\alpha,-1}_{k+1} x_p + \hat K^{\alpha,-1}_{k+1} \left[ h \gamma (W^{\alpha}_{k+1})^{-1}    B^{\alpha}_{k+1} \lambda^{\alpha+1}_{k+1}\right]}   \end{array}\end{equation}\begin{ndrva}  Olivier: Could you confirm the definition of $x_q$ ?\end{ndrva}\paragraph{Reduction to a linear relation between  $y^{\alpha+1}_{k+\gamma}$ and$\lambda^{\alpha+1}_{k+\gamma}$}Inserting (\ref{eq:full-rfree-13}) into (\ref{eq:full-NL11y}), we get the following linear relation between $y^{\alpha+1}_{k+1}$ and $\lambda^{\alpha+1}_{k+1}$, \begin{equation}   \begin{array}{l} y^{\alpha+1}_{k+1} = y_p + \left[ h  C^{\alpha}_{k+1} (\tilde K^{\alpha}_{k+1})^{-1}( W^{\alpha}_{k+1})^{-1}  B^{\alpha}_{k+1} + D^{\alpha}_{k+1} \right]\lambda^{\alpha+1}_{k+1}   \end{array}\end{equation}with \begin{equation}\boxed{y_p = y^{\alpha}_{k+1} -\mathcal R^{\alpha}_{yk+1} + C^{\alpha}_{k+1}(x_q) -D^{\alpha}_{k+1} \lambda^{\alpha}_{k+1} }\end{equation}\textcolor{red}{  \begin{equation}   \boxed{ x_q=(\tilde K^{\alpha}_{k+1})^{-1}x_p -x^{\alpha}_{k+1})\label{eq:full-xqq}}  \end{equation}}\clearpage%%% Local Variables: %%% mode: latex%%% TeX-master: "DevNotes"%%% End: 