\section{Newton's linearization of~(\ref{first-DS2})} Let us now proceed with the time discretization of (\ref{first-DS2}) by a fully implicit scheme : \begin{equation}  \begin{array}{l}    \label{eq:mlcp2-toto1-DS2}     M x_{k+1} = M x_{k} +h\theta f(x_{k+1},t_{k+1})+h(1-\theta) f(x_k,t_k) + h \gamma r(t_{k+1})     + h(1-\gamma)r(t_k)  \\[2mm]     y_{k+1} =  h(t_{k+1},x_{k+1},\lambda _{k+1}) \\[2mm]     r_{k+1} = g(\lambda_{k+1},t_{k+1})\\[2mm]  \end{array}\end{equation} \paragraph{Newton's linearization of the first line of~(\ref{eq:mlcp2-toto-DS2})} The first line of the  problem~(\ref{eq:mlcp2-toto-DS2}) can be written under the form of a residue $\mathcal R$ depending only on $x_{k+1}$ and $r_{k+1}$ such that \begin{equation}  \label{eq:mlcp2-NL3}  \mathcal R (x_{k+1},r _{k+1}) =0\end{equation}with $\mathcal R(x,r) = M(x - x_{k}) -h\theta f( x , t_{k+1}) - h(1-\theta)f(x_k,t_k) - h\gamma r- h(1-\gamma)r_k$.The solution of this system of nonlinear equations is sought as a limit of the sequence $\{ x^{\alpha}_{k+1},r^{\alpha}_{k+1} \}_{\alpha \in \NN}$ such that \begin{equation}   \label{eq:mlcp2-NL7}   \begin{cases}     x^{0}_{k+1} = x_k \\ \\     \mathcal R_L( x^{\alpha+1}_{k+1},r^{\alpha+1}_{k+1}) = \mathcal     R(x^{\alpha}_{k+1},r^{\alpha}_{k+1})  + \left[ \nabla_{x} \mathcal     R(x^{\alpha}_{k+1},r^{\alpha}_{k+1})\right] (x^{\alpha+1}_{k+1}-x^{\alpha}_{k+1} ) +     \left[ \nabla_{r} \mathcal R(x^{\alpha}_{k+1},r^{\alpha}_{k+1})\right] (r^{\alpha+1}_{k+1} - r^{\alpha}_{k+1} ) =0 \end{cases}\end{equation}\begin{ndrva}  What about $r^0_{k+1}$ ?\end{ndrva}The residu free is also defined (useful for implementation only):\[\mathcal R _{free}(x) \stackrel{\Delta}{=}  M(x - x_{k}) -h\theta f( x , t_{k+1}) - h(1-\theta)f(x_k,t_k),\]which yields\[\mathcal R (x,r) = \mathcal R _{free}(x)   - h\gamma r - h(1-\gamma)r_k.\]\begin{equation}  \mathcal R (x^{\alpha}_{k+1},r^{\alpha}_{k+1}) = \fbox{$\mathcal R^{\alpha}_{k+1} \stackrel{\Delta}{=}  \mathcal R_{free}(x^{\alpha}_{k+1},r^{\alpha}_{k+1} )  - h\gamma r^{\alpha}_{k+1} - h(1-\gamma)r_k$}\label{eq:mlcp2-rfree-1}\end{equation}\[  \mathcal R_{free}(x^{\alpha}_{k+1},r^{\alpha}_{k+1} )=\fbox{$ \mathcal R _{free k+1} ^{\alpha} \stackrel{\Delta}{=}  M(x^{\alpha}_{k+1} - x_{k}) -h\theta f( x^{\alpha}_{k+1} , t_{k+1}) - h(1-\theta)f(x_k,t_k)$}\] The computation of the Jacobian of $\mathcal R$ with respect to $x$, denoted by $   W^{\alpha}_{k+1}$ leads to \begin{equation}   \label{eq:mlcp2-NL9}   \begin{array}{l}    W^{\alpha}_{k+1} \stackrel{\Delta}{=} \nabla_{x} \mathcal R (x^{\alpha}_{k+1},r^{\alpha}_{k+1})= M - h  \theta \nabla_{x} f(  x^{\alpha}_{k+1}, t_{k+1} ).\\ \end{array}\end{equation}At each time--step, we have to solve the following linearized problem,\begin{equation}   \label{eq:mlcp2-NL10}    \mathcal R^{\alpha}_{k+1} + W^{\alpha}_{k+1} (x^{\alpha+1}_{k+1} -    x^{\alpha}_{k+1}) - h \gamma (r^{\alpha+1}_{k+1} - r^{\alpha}_{k+1} )  =0 ,\end{equation}By using (\ref{eq:mlcp2-rfree-1}), we get\begin{equation}  \label{eq:mlcp2-rfree-2}  \mathcal R_{free}(x^{\alpha}_{k+1},r^{\alpha}_{k+1} )  - h\gamma r^{\alpha+1}_{k+1} - h(1-\gamma)r_k  + W^{\alpha}_{k+1} (x^{\alpha+1}_{k+1} -    x^{\alpha}_{k+1})  =0 \end{equation}%\fbox{  \begin{equation}    \boxed{ x^{\alpha+1}_{k+1} = h(W^{\alpha}_{k+1})^{-1}r^{\alpha+1}_{k+1} +x^\alpha_{free}}  \end{equation}}with :\begin{equation}  \boxed{x^\alpha_{free}\stackrel{\Delta}{=}x^{\alpha}_{k+1}-(W^{\alpha}_{k+1})^{-1}\mathcal (R_{freek+1}^{\alpha} \textcolor{red}{- h(1-\gamma) r_k})\label{eq:mlcp2-rfree-12}}\end{equation}The matrix $W$ is clearly non singular for small $h$.% that is% \begin{equation}%    \begin{array}{l}%  h \gamma  r^{\alpha+1}_{k+1} = r_c + W^{\alpha}_{k+1} x^{\alpha+1}_{k+1}%  .\label{eq:mlcp2-NL11} %  \end{array}% \end{equation}% with % \begin{equation}%    \begin{array}{l}% r_c \stackrel{\Delta}{=} h \gamma r^{\alpha}_{k+1} - W^{\alpha}_{k+1} x^{\alpha}_{k+1} + \mathcal R% ^{\alpha}_{k+1}=- W^{\alpha}_{k+1} x^{\alpha}_{k+1} + \mathcal R_{free k+1} ^{\alpha} - h(1-\gamma)r_k\\ \\% \end{array}% \end{equation}% \begin{equation}%    \begin{array}{l}% \mathcal R ^{\alpha}_{k+1}=M( x^{\alpha}_{k+1} - x_k) -h \theta f(x^{\alpha}_{k+1})-h(1-\theta)f(x_k)% - h \gamma r^{\alpha}_{k+1} -h(1- \gamma)r_k%  \end{array}%    \end{equation}% \[x^{\alpha+1}_{k+1} = h(W^{\alpha}_{k+1})^{-1}r^{\alpha+1}_{k+1} +(W^{\alpha}_{k+1})^{-1}(\mathcal% R_{free k+1} ^{\alpha})+x^{\alpha}_{k+1}\] \paragraph{Newton's linearization of the second  line of~(\ref{eq:mlcp2-toto1-DS2})}The same operation is performed with the second equation of (\ref{eq:mlcp2-toto1-DS2})\begin{equation}  \begin{array}{l}    \mathcal R_y(x,y,\lambda)=y-h(t_{k+1},x,\lambda) =0\\ \\  \end{array}\end{equation}which is linearized as\begin{equation}  \label{eq:mlcp2-NL9}  \begin{array}{l}    \mathcal R_{Ly}(x^{\alpha+1}_{k+1},y^{\alpha+1}_{k+1},\lambda^{\alpha+1}_{k+1}) = \mathcal    R_{y}(x^{\alpha}_{k+1},y^{\alpha}_{k+1},\lambda^{\alpha}_{k+1}) +    (y^{\alpha+1}_{k+1}-y^{\alpha}_{k+1})- \\[2mm] \qquad  \qquad \qquad \qquad  \qquad \qquad    C^{\alpha}_{k+1}(x^{\alpha+1}_{k+1}-x^{\alpha}_{k+1}) - D^{\alpha}_{k+1}(\lambda^{\alpha+1}_{k+1}-\lambda^{\alpha}_{k+1})=0  \end{array}\end{equation}This leads to the following linear equation\begin{equation}  \boxed{y^{\alpha+1}_{k+1} =  y^{\alpha}_{k+1}  -\mathcal R^{\alpha}_{yk+1}+ \\  C^{\alpha}_{k+1}(x^{\alpha+1}_{k+1}-x^{\alpha}_{k+1}) +  D^{\alpha}_{k+1}(\lambda^{\alpha+1}_{k+1}-\lambda^{\alpha}_{k+1})}. \label{eq:mlcp2-NL11y}\end{equation}with,\begin{equation}     \begin{array}{l}  C^{\alpha}_{k+1} = \nabla_xh(t_{k+1}, x^{\alpha}_{k+1},\lambda^{\alpha}_{k+1} ) \\ \\  D^{\alpha}_{k+1} = \nabla_{\lambda}h(t_{k+1}, x^{\alpha}_{k+1},\lambda^{\alpha}_{k+1}) \end{array}\end{equation}and\begin{equation}\fbox{$\mathcal R^{\alpha}_{yk+1} \stackrel{\Delta}{=} y^{\alpha}_{k+1} - h(x^{\alpha}_{k+1},\lambda^{\alpha}_{k+1})$} \end{equation} \paragraph{Newton's linearization of the third  line of~(\ref{eq:mlcp2-toto1-DS2})}The same operation is performed with the third equation of (\ref{eq:mlcp2-toto1-DS2})\begin{equation}  \begin{array}{l}    \mathcal R_r(r,x,\lambda)=r-g(\lambda,t_{k+1}) =0\\ \\  \end{array}\end{equation}which is linearized as\begin{equation}  \label{eq:mlcp2-NL9}  \begin{array}{l}      \mathcal R_{L\lambda}(r^{\alpha+1}_{k+1},x^{\alpha+1}_{k+1},\lambda^{\alpha+1}_{k+1}) = \mathcal      R_{rk+1}^{\alpha} + (r^{\alpha+1}_{k+1} - r^{\alpha}_{k+1}) - B^{\alpha}_{k+1}(\lambda^{\alpha+1}_{k+1} -      \lambda^{\alpha}_{k+1})=0    \end{array}  \end{equation}\begin{equation}  \label{eq:mlcp2-rrL}  \begin{array}{l}    \boxed{r^{\alpha+1}_{k+1} = g(x ^{\alpha}_{k+1},\lambda ^{\alpha}_{k+1},t_{k+1}) -B^{\alpha}_{k+1}      \lambda^{\alpha}_{k+1} + B^{\alpha}_{k+1} \lambda^{\alpha+1}}         \end{array}\end{equation}with,\begin{equation}     \begin{array}{l}  B^{\alpha}_{k+1} = \nabla_{\lambda}g(x^{\alpha}_{k+1},\lambda ^{\alpha}_{k+1},t_{k+1}) \end{array}\end{equation}and the  residue for $r$:\begin{equation}\boxed{\mathcal      R_{rk+1}^{\alpha} = r^{\alpha}_{k+1} - g(\lambda ^{\alpha}_{k+1},t_{k+1})}  \end{equation}\paragraph{Reduction to a linear relation between  $x^{\alpha+1}_{k+1}$ and$\lambda^{\alpha+1}_{k+1}$}Inserting (\ref{eq:mlcp2-rrL}) into~(\ref{eq:mlcp2-rfree-12}), we get the following linear relation between $x^{\alpha+1}_{k+1}$ and$\lambda^{\alpha+1}_{k+1}$, \begin{equation}   \begin{array}{l}     x^{\alpha+1}_{k+1} = h\gamma(W^{\alpha}_{k+1} )^{-1}\left[g(x^{\alpha}_{k+1},\lambda^{\alpha}_{k+1},t_{k+1}) +    B^{\alpha}_{k+1} (\lambda^{\alpha+1}_{k+1} - \lambda^{\alpha}_{k+1}) \right ] +x^\alpha_{free}\end{array}\end{equation}that is \begin{equation}  \begin{array}{l}   x^{\alpha+1}_{k+1} =x_p + h \gamma (W^{\alpha}_{k+1})^{-1}    B^{\alpha}_{k+1} \lambda^{\alpha+1}_{k+1}   \end{array}\end{equation}with \begin{equation}  \boxed{x_p \stackrel{\Delta}{=}  h\gamma(W^{\alpha}_{k+1} )^{-1}\left[g(x^{\alpha}_{k+1},\lambda^{\alpha}_{k+1},t_{k+1}) +    -B^{\alpha}_{k+1} (\lambda^{\alpha}_{k+1}) \right ] +x^\alpha_{free}}\end{equation}We get the linear relation\begin{equation}  \label{eq:mlcp2-rfree-13}  \begin{array}{l} \boxed{   x^{\alpha+1}_{k+1}\stackrel{\Delta}{=} x_p + \left[ h \gamma (W^{\alpha}_{k+1})^{-1}    B^{\alpha}_{k+1} \lambda^{\alpha+1}_{k+1}\right]}   \end{array}\end{equation}\paragraph{Reduction to a linear relation between  $y^{\alpha+1}_{k+1}$ and$\lambda^{\alpha+1}_{k+1}$}Inserting (\ref{eq:mlcp2-rfree-13}) into (\ref{eq:mlcp2-NL11y}), we get the following linear relation between $y^{\alpha+1}_{k+1}$ and $\lambda^{\alpha+1}_{k+1}$, \begin{equation}   \begin{array}{l} y^{\alpha+1}_{k+1} = y_p + \left[ h  C^{\alpha}_{k+1} ( W^{\alpha}_{k+1})^{-1}  B^{\alpha}_{k+1} + D^{\alpha}_{k+1} \right]\lambda^{\alpha+1}_{k+1}   \end{array}\end{equation}with \begin{equation}\boxed{y_p = y^{\alpha}_{k+1} -\mathcal R^{\alpha}_{yk+1} + C^{\alpha}_{k+1}(x_q) -D^{\alpha}_{k+1} \lambda^{\alpha}_{k+1} }\end{equation}\textcolor{red}{  \begin{equation}    \boxed{ x_q= x_p - x^{\alpha}_{k+1}\label{eq:mlcp2-xqq}}  \end{equation}}\clearpage%%% Local Variables: %%% mode: latex%%% TeX-master: "DevNotes"%%% End: 